C-verifier/src/Midend-IVL/Isabelle-UTP-Extended/hoare/HoareLogic/PartialCorrectness/utp_hoare.thy
@@ -4,8 +4,16 @@ theory utp_hoare
 imports "../../AlgebraicLaws/Rel&Des/Algebraic_Laws"
 begin
 
-named_theorems hoare
+named_theorems hoare and hoare_safe
 
+method hoare_split uses hr = 
+  ((simp add: assigns_r_comp usubst unrest)?, -- {* Eliminate assignments where possible *}
+   (auto 
+    intro: hoare intro!: hoare_safe hr
+    simp add: assigns_r_comp conj_comm conj_assoc usubst unrest))[1] -- {* Apply Hoare logic laws *}
+
+method hoare_auto uses hr = (hoare_split hr: hr; rel_auto?)
+  
 subsection {*Hoare triple definition*}
 
 text {*A Hoare triple is represented by a pre-condition @{text P} a post-condition @{text Q}
@@ -54,12 +62,12 @@ lemma hoare_r_conj [hoare]:
 
 subsection {*Hoare SKIP*}
 
-lemma skip_hoare_r [hoare]: "\<lbrace>p\<rbrace>II\<lbrace>p\<rbrace>\<^sub>u"
+lemma skip_hoare_r [hoare_safe]: "\<lbrace>p\<rbrace>II\<lbrace>p\<rbrace>\<^sub>u"
   by rel_auto
 
 subsection {*Hoare for assignment*}
 
-lemma assigns_hoare_r [hoare]:
+lemma assigns_hoare_r [hoare_safe]:
   assumes"`p \<Rightarrow> \<sigma> \<dagger> q`"
   shows  "\<lbrace>p\<rbrace>\<langle>\<sigma>\<rangle>\<^sub>a\<lbrace>q\<rbrace>\<^sub>u"
   by (insert assms) rel_auto
@@ -87,21 +95,51 @@ lemma assigns_floyd_r [hoare]:
 
 subsection {*Hoare for Sequential Composition*}
 
-lemma seq_hoare_r [hoare]:
+lemma seq_hoare_r:
   assumes"\<lbrace>p\<rbrace>C\<^sub>1\<lbrace>s\<rbrace>\<^sub>u" and "\<lbrace>s\<rbrace>C\<^sub>2\<lbrace>r\<rbrace>\<^sub>u"
   shows"\<lbrace>p\<rbrace>C\<^sub>1 ;; C\<^sub>2\<lbrace>r\<rbrace>\<^sub>u"
   by (insert assms) rel_auto
+    
+lemma seq_hoare_invariant [hoare_safe]: 
+  assumes "\<lbrace>p\<rbrace>Q\<^sub>1\<lbrace>p\<rbrace>\<^sub>u" and "\<lbrace>p\<rbrace>Q\<^sub>2\<lbrace>p\<rbrace>\<^sub>u" 
+  shows "\<lbrace>p\<rbrace>Q\<^sub>1 ;; Q\<^sub>2\<lbrace>p\<rbrace>\<^sub>u"
+  using assms 
+  by (auto simp: seq_hoare_r)
 
+lemma seq_hoare_stronger_pre_1 [hoare_safe]: 
+  assumes "\<lbrace>p \<and> q\<rbrace>Q\<^sub>1\<lbrace>p \<and> q\<rbrace>\<^sub>u" and "\<lbrace>p \<and> q\<rbrace>Q\<^sub>2\<lbrace>q\<rbrace>\<^sub>u" 
+  shows "\<lbrace>p \<and> q\<rbrace>Q\<^sub>1 ;; Q\<^sub>2\<lbrace>q\<rbrace>\<^sub>u"
+  using assms 
+  by (auto simp: seq_hoare_r)
+
+lemma seq_hoare_stronger_pre_2 [hoare_safe]: 
+  assumes "\<lbrace>p \<and> q\<rbrace>Q\<^sub>1\<lbrace>p \<and> q\<rbrace>\<^sub>u" and "\<lbrace>p \<and> q\<rbrace>Q\<^sub>2\<lbrace>p\<rbrace>\<^sub>u" 
+  shows "\<lbrace>p \<and> q\<rbrace>Q\<^sub>1 ;; Q\<^sub>2\<lbrace>p\<rbrace>\<^sub>u"
+  using assms 
+  by (auto simp: seq_hoare_r)
+   
+lemma seq_hoare_inv_r_2 [hoare]: 
+  assumes "\<lbrace>p\<rbrace>Q\<^sub>1\<lbrace>q\<rbrace>\<^sub>u" and "\<lbrace>q\<rbrace>Q\<^sub>2\<lbrace>q\<rbrace>\<^sub>u" 
+  shows   "\<lbrace>p\<rbrace>Q\<^sub>1 ;; Q\<^sub>2\<lbrace>q\<rbrace>\<^sub>u"
+  using assms 
+  by (auto simp: seq_hoare_r)
+ 
+lemma seq_hoare_inv_r_3 [hoare]: 
+  assumes "\<lbrace>p\<rbrace>Q\<^sub>1\<lbrace>p\<rbrace>\<^sub>u" and "\<lbrace>p\<rbrace>Q\<^sub>2\<lbrace>q\<rbrace>\<^sub>u" 
+  shows "\<lbrace>p\<rbrace>Q\<^sub>1 ;; Q\<^sub>2\<lbrace>q\<rbrace>\<^sub>u"
+  using assms 
+  by (auto simp: seq_hoare_r)
+    
 subsection {*Hoare for Conditional*}
 
-lemma cond_hoare_r [hoare]: 
+lemma cond_hoare_r [hoare_safe]: 
   assumes "\<lbrace>b \<and> p\<rbrace>C\<^sub>1\<lbrace>q\<rbrace>\<^sub>u" and "\<lbrace>\<not>b \<and> p\<rbrace>C\<^sub>2\<lbrace>q\<rbrace>\<^sub>u" 
   shows "\<lbrace>p\<rbrace>C\<^sub>1 \<triangleleft> b \<triangleright>\<^sub>r C\<^sub>2\<lbrace>q\<rbrace>\<^sub>u"
   by (insert assms) rel_auto
 
 subsection {*Hoare for assert*}
 
-lemma assert_hoare_r [hoare]: 
+lemma assert_hoare_r [hoare_safe]: 
   assumes "\<lbrace>c \<and> p\<rbrace>II\<lbrace>q\<rbrace>\<^sub>u" and "\<lbrace>\<not>c \<and> p\<rbrace>true\<lbrace>q\<rbrace>\<^sub>u" 
   shows "\<lbrace>p\<rbrace>c\<^sub>\<bottom>\<lbrace>q\<rbrace>\<^sub>u"
   unfolding rassert_def using assms cond_hoare_r [of c p _ q ]
@@ -109,7 +147,7 @@ lemma assert_hoare_r [hoare]:
 
 subsection {*Hoare for assume*}
 
-lemma assume_hoare_r [hoare]: 
+lemma assume_hoare_r [hoare_safe]: 
   assumes "\<lbrace>c \<and> p\<rbrace>II\<lbrace>q\<rbrace>\<^sub>u" and "\<lbrace>\<not>c \<and> p\<rbrace>false\<lbrace>q\<rbrace>\<^sub>u" 
   shows "\<lbrace>p\<rbrace>c\<^sup>\<top>\<lbrace>q\<rbrace>\<^sub>u"
   unfolding rassume_def using assms cond_hoare_r [of c p _ q ]
@@ -117,24 +155,39 @@ lemma assume_hoare_r [hoare]:
 
 subsection {*Hoare for While-loop*}
 
-lemma while_hoare_r [hoare]:
+lemma while_hoare_r [hoare_safe]:
   assumes "\<lbrace>p \<and> b\<rbrace>C\<lbrace>p\<rbrace>\<^sub>u"
   shows "\<lbrace>p\<rbrace>while b do C od\<lbrace>\<not>b \<and> p\<rbrace>\<^sub>u"
   using assms
   apply (simp add: while_def hoare_r_def)apply ( rule_tac lfp_lowerbound) apply(rel_auto)
   done
-lemma while_hoare_r' [hoare]:
+
+lemma while_hoare_r' [hoare_safe]:
   assumes "\<lbrace>p \<and> b\<rbrace>C\<lbrace>p\<rbrace>\<^sub>u" and "`p \<and> \<not>b \<Rightarrow> q`"
   shows "\<lbrace>p\<rbrace>while b do C od\<lbrace>q\<rbrace>\<^sub>u"
   using assms
   by (metis conj_comm hoare_r_conseq p_imp_p taut_true while_hoare_r)
 
 
-lemma while_invr_hoare_r [hoare]:
+lemma while_invr_hoare_r  [hoare_safe]:
   assumes "\<lbrace>p \<and> b\<rbrace>C\<lbrace>p\<rbrace>\<^sub>u" and "`pre \<Rightarrow> p`" and "`(\<not>b \<and> p) \<Rightarrow> post`"
   shows "\<lbrace>pre\<rbrace>while b invr p do C od\<lbrace>post\<rbrace>\<^sub>u"
   by (metis assms hoare_r_conseq while_hoare_r while_inv_def)
 
 
+text {* Frame rule: If starting $S$ in a state satisfying $p establishes q$ in the final state, then
+  we can insert an invariant predicate $r$ when $S$ is framed by $a$, provided that $r$ does not
+  refer to variables in the frame, and $q$ does not refer to variables outside the frame. *}
+    
+lemma frame_hoare_r [hoare_safe]: 
+  assumes "vwb_lens a" "a \<sharp> r" "a \<natural> q" "\<lbrace>p \<and> r\<rbrace>S\<lbrace>q\<rbrace>\<^sub>u"
+  shows "\<lbrace>p \<and> r\<rbrace>a:[S]\<lbrace>q \<and> r\<rbrace>\<^sub>u"
+  using assms by (rel_simp)
+
+lemma frame_hoare_r' [hoare_safe]: 
+  assumes "vwb_lens a" "a \<sharp> r" "a \<natural> q" "\<lbrace>r \<and> p\<rbrace>S\<lbrace>q\<rbrace>\<^sub>u"
+  shows "\<lbrace>r \<and> p\<rbrace>a:[S]\<lbrace>r \<and> q\<rbrace>\<^sub>u"
+  using assms
+  by (simp add: frame_hoare_r utp_pred_laws.inf.commute)    
 
 end
